Prove sim_configuration_certify

src/localdrf/TimeTraced.v
@@ -174,3 +174,31 @@ Proof.
     { i. eapply join_well_ordered; eauto. }
   }
 Qed.
+
+Inductive times_configuration_opt_step (times: Loc.t -> Time.t -> Prop)
+  : forall lang (tr tr_cert: Trace.t lang)
+           (e:MachineEvent.t) (tid:Ident.t) (c1 c2:Configuration.t), Prop :=
+| times_configuration_opt_step_some
+    lang tr tr_cert e tid c1 c2
+    (STEP: @times_configuration_step times lang tr tr_cert e tid c1 c2)
+  :
+    times_configuration_opt_step times tr tr_cert e tid c1 c2
+| times_configuration_opt_step_none
+    lang tid c
+  :
+    @times_configuration_opt_step times lang [] [] MachineEvent.silent tid c c
+.
+
+Lemma times_configuration_opt_step_future
+      times lang tr tr_cert e tid c1 c2
+      (STEP: @times_configuration_opt_step times lang tr tr_cert e tid c1 c2)
+      (WF1: Configuration.wf c1):
+  (<<WF2: Configuration.wf c2>>) /\
+  (<<SC_FUTURE: TimeMap.le c1.(Configuration.sc) c2.(Configuration.sc)>>) /\
+  (<<MEM_FUTURE: Memory.future c1.(Configuration.memory) c2.(Configuration.memory)>>).
+Proof.
+  inv STEP.
+  { apply inj_pair2 in H1. apply inj_pair2 in H2. subst.
+    eapply times_configuration_step_future; eauto. }
+  { apply inj_pair2 in H1. apply inj_pair2 in H2. subst. splits; auto. refl. }
+Qed.
